alloc_and_blit in the buffer library with all the flavors of alloc

ulib/LowStar.ImmutableBuffer.fst
@@ -45,105 +45,159 @@ inline_for_extraction let isub (#a:Type0) = msub #a #(immutable_preorder a) #(im
 
 inline_for_extraction let ioffset (#a:Type0) = moffset #a #(immutable_preorder a) #(immutable_preorder a) (immutable_preorder a)
 
-let cpred (#a:Type0) (s:Seq.seq a) :spred a = fun s1 -> Seq.equal s s1
+(*
+ * Shorthand for erased sequence
+ *)
+type eseq (a:Type) = G.erased (Seq.seq a)
 
-unfold let libuffer (a:Type0) (len:nat) (s:Seq.seq a) =
-  b:lmbuffer a (immutable_preorder a) (immutable_preorder a) len{witnessed b (cpred s)}
+let cpred (#a:Type0) (s:eseq a) :spred a = fun s1 -> Seq.equal (G.reveal s) s1
 
-unfold let libuffer_or_null (a:Type0) (len:nat) (r:HS.rid) (s:Seq.seq a) =
+let value_is #a (b:ibuffer a) (s:eseq a) =
+  witnessed b (cpred s)
+
+unfold let libuffer (a:Type0) (len:nat) (s:eseq a) =
+  b:lmbuffer a (immutable_preorder a) (immutable_preorder a) len{b `value_is` s}
+
+unfold let libuffer_or_null (a:Type0) (len:nat) (r:HS.rid) (s:eseq a) =
   b:lmbuffer_or_null a (immutable_preorder a) (immutable_preorder a) len r{(not (g_is_null b)) ==>
-                                                                           witnessed b (cpred s)}
+                                                                           b `value_is` s}
 
 let igcmalloc (#a:Type0) (r:HS.rid) (init:a) (len:U32.t)
-  :HST.ST (b:libuffer a (U32.v len) (Seq.create (U32.v len) init){frameOf b == r /\ recallable b})
+  :HST.ST (b:libuffer a (U32.v len) (G.hide (Seq.create (U32.v len) init)){frameOf b == r /\ recallable b})
           (requires (fun _       -> malloc_pre r len))
           (ensures  (fun h0 b h1 -> alloc_post_mem_common b h0 h1 (Seq.create (U32.v len) init)))
   = let b = mgcmalloc r init len in
-    witness_p b (cpred (Seq.create (U32.v len) init));
+    witness_p b (cpred (G.hide (Seq.create (U32.v len) init)));
+    b
+
+(*
+ * Unlike other allocation functions in this module,
+ *   this function (and other flavors of alloc_and_blit) don't provide the witnessed contents
+ *   as the refinement of the return type
+ * This is because the contents depend on the input memory (== the contents of src)
+ *)
+let igcmalloc_and_blit (#a:Type0) (r:HS.rid)
+  (#rrel1 #rel1:srel a) (src:mbuffer a rrel1 rel1) (id_src:U32.t) (len:U32.t)
+  : HST.ST (b:lmbuffer a (immutable_preorder a) (immutable_preorder a) (U32.v len){frameOf b == r})
+    (requires fun h0 ->
+      malloc_pre r len /\
+      live h0 src /\ U32.v id_src + U32.v len <= length src)
+    (ensures fun h0 b h1 ->
+      let s = Seq.slice (as_seq h0 src) (U32.v id_src) (U32.v id_src + U32.v len) in
+      alloc_post_mem_common b h0 h1 s /\
+      b `value_is` G.hide s)
+  = let b = mgcmalloc_and_blit r src id_src len in
+    let h0 = HST.get () in
+    witness_p b (cpred (G.hide (Seq.slice (as_seq h0 src) (U32.v id_src) (U32.v id_src + U32.v len))));
     b
 
 inline_for_extraction
 let igcmalloc_partial (#a:Type0) (r:HS.rid) (init:a) (len:U32.t)
-  :HST.ST (b:libuffer_or_null a (U32.v len) r (Seq.create (U32.v len) init){recallable b})
+  :HST.ST (b:libuffer_or_null a (U32.v len) r (G.hide (Seq.create (U32.v len) init)){recallable b})
           (requires (fun _       -> malloc_pre r len))
           (ensures  (fun h0 b h1 -> alloc_partial_post_mem_common b h0 h1 (Seq.create (U32.v len) init)))
   = igcmalloc r init len
 
 let imalloc (#a:Type0) (r:HS.rid) (init:a) (len:U32.t)
-  :HST.ST (b:libuffer a (U32.v len) (Seq.create (U32.v len) init){frameOf b == r /\ freeable b})
+  :HST.ST (b:libuffer a (U32.v len) (G.hide (Seq.create (U32.v len) init)){frameOf b == r /\ freeable b})
           (requires (fun _       -> malloc_pre r len))
           (ensures  (fun h0 b h1 -> alloc_post_mem_common b h0 h1 (Seq.create (U32.v len) init)))
   = let b = mmalloc r init len in
-    witness_p b (cpred (Seq.create (U32.v len) init));
+    witness_p b (cpred (G.hide (Seq.create (U32.v len) init)));
+    b
+
+let imalloc_and_blit (#a:Type0) (r:HS.rid)
+  (#rrel1 #rel1:srel a) (src:mbuffer a rrel1 rel1) (id_src:U32.t) (len:U32.t)
+  : HST.ST (b:lmbuffer a (immutable_preorder a) (immutable_preorder a) (U32.v len){frameOf b == r /\ freeable b})
+    (requires fun h0 ->
+      malloc_pre r len /\
+      live h0 src /\ U32.v id_src + U32.v len <= length src)
+    (ensures fun h0 b h1 ->
+      let s = Seq.slice (as_seq h0 src) (U32.v id_src) (U32.v id_src + U32.v len) in
+      alloc_post_mem_common b h0 h1 s /\
+      b `value_is` G.hide s)
+  = let b = mmalloc_and_blit r src id_src len in
+    let h0 = HST.get () in
+    witness_p b (cpred (G.hide (Seq.slice (as_seq h0 src) (U32.v id_src) (U32.v id_src + U32.v len))));
     b
 
 inline_for_extraction
 let imalloc_partial (#a:Type0) (r:HS.rid) (init:a) (len:U32.t)
-  :HST.ST (b:libuffer_or_null a (U32.v len) r (Seq.create (U32.v len) init){(not (g_is_null b)) ==> freeable b})
+  :HST.ST (b:libuffer_or_null a (U32.v len) r (G.hide (Seq.create (U32.v len) init)){(not (g_is_null b)) ==> freeable b})
           (requires (fun _       -> malloc_pre r len))
           (ensures  (fun h0 b h1 -> alloc_partial_post_mem_common b h0 h1 (Seq.create (U32.v len) init)))
   = imalloc r init len
 
 let ialloca (#a:Type0) (init:a) (len:U32.t)
-  :HST.StackInline (libuffer a (U32.v len) (Seq.create (U32.v len) init))
+  :HST.StackInline (libuffer a (U32.v len) (G.hide (Seq.create (U32.v len) init)))
                    (requires (fun _       -> alloca_pre len))
                    (ensures  (fun h0 b h1 -> alloc_post_mem_common b h0 h1 (Seq.create (U32.v len) init) /\
 		                          frameOf b == HS.get_tip h0))
   = let b = malloca init len in
-    witness_p b (cpred (Seq.create (U32.v len) init));
+    witness_p b (cpred (G.hide (Seq.create (U32.v len) init)));
+    b
+
+let ialloca_and_blit (#a:Type0)
+  (#rrel1 #rel1:srel a) (src:mbuffer a rrel1 rel1) (id_src:U32.t) (len:U32.t)
+  : HST.StackInline (b:lmbuffer a (immutable_preorder a) (immutable_preorder a) (U32.v len))
+    (requires fun h0 ->
+      alloca_pre len /\
+      live h0 src /\ U32.v id_src + U32.v len <= length src)
+    (ensures fun h0 b h1 ->
+      let s = Seq.slice (as_seq h0 src) (U32.v id_src) (U32.v id_src + U32.v len) in
+      alloc_post_mem_common b h0 h1 s /\
+      frameOf b == HS.get_tip h0 /\
+      b `value_is` G.hide s)
+  = let b = malloca_and_blit src id_src len in
+    let h0 = HST.get () in
+    witness_p b (cpred (G.hide (Seq.slice (as_seq h0 src) (U32.v id_src) (U32.v id_src + U32.v len))));
     b
 
 let ialloca_of_list (#a:Type0) (init: list a)
-  :HST.StackInline (b:libuffer a (normalize_term (List.Tot.length init)) (Seq.seq_of_list init))
+  :HST.StackInline (b:libuffer a (normalize_term (List.Tot.length init)) (G.hide (Seq.seq_of_list init)))
                    (requires (fun _      -> alloca_of_list_pre init))
                    (ensures (fun h0 b h1 -> alloc_post_mem_common b h0 h1 (Seq.seq_of_list init) /\
 		                         frameOf b == HS.get_tip h0))
   = let b = malloca_of_list init in
-    witness_p b (cpred (Seq.seq_of_list init));
+    witness_p b (cpred (G.hide (Seq.seq_of_list init)));
     b
 
 let igcmalloc_of_list (#a:Type0) (r:HS.rid) (init:list a)
-  :HST.ST (b:libuffer a (normalize_term (List.Tot.length init)) (Seq.seq_of_list init){frameOf b == r /\ recallable b})
+  :HST.ST (b:libuffer a (normalize_term (List.Tot.length init)) (G.hide (Seq.seq_of_list init)){frameOf b == r /\ recallable b})
           (requires (fun _       -> gcmalloc_of_list_pre r init))
           (ensures  (fun h0 b h1 -> alloc_post_mem_common b h0 h1 (Seq.seq_of_list init)))
   = let b = mgcmalloc_of_list r init in
-    witness_p b (cpred (Seq.seq_of_list init));
+    witness_p b (cpred (G.hide (Seq.seq_of_list init)));
     b
 
 inline_for_extraction
 let igcmalloc_of_list_partial (#a:Type0) (r:HS.rid) (init:list a)
-  :HST.ST (b:libuffer_or_null a (normalize_term (List.Tot.length init)) r (Seq.seq_of_list init){recallable b})
+  :HST.ST (b:libuffer_or_null a (normalize_term (List.Tot.length init)) r (G.hide (Seq.seq_of_list init)){recallable b})
           (requires (fun _       -> gcmalloc_of_list_pre r init))
           (ensures  (fun h0 b h1 -> alloc_partial_post_mem_common b h0 h1 (Seq.seq_of_list init)))
   = igcmalloc_of_list r init
 
 let witness_contents (#a:Type0) (b:ibuffer a) (s:Seq.seq a)
   :HST.ST unit (requires (fun h0        -> Seq.equal (as_seq h0 b) s))
-                 (ensures  (fun h0 _ h1 -> h0 == h1 /\ witnessed b (cpred s)))
-  = witness_p b (cpred s)
+                 (ensures  (fun h0 _ h1 -> h0 == h1 /\ b `value_is` G.hide s))
+  = witness_p b (cpred (G.hide s))
 
 let recall_contents (#a:Type0) (b:ibuffer a) (s:Seq.seq a)
-  :HST.ST unit (requires (fun h0      -> (recallable b \/ live h0 b) /\ witnessed b (cpred s)))
+  :HST.ST unit (requires (fun h0      -> (recallable b \/ live h0 b) /\ b `value_is` G.hide s))
                (ensures  (fun h0 _ h1 -> h0 == h1 /\ live h0 b /\ as_seq h0 b == s))
-  = recall_p b (cpred s)
-
-let seq_eq (s:Ghost.erased (Seq.seq 'a)) (s':Seq.seq 'a) =
-  s' `Seq.equal` Ghost.reveal s
-  
-let value_is #a (b:ibuffer a) (s:Ghost.erased (Seq.seq a)) =
-  witnessed b (seq_eq s)
+  = recall_p b (cpred (G.hide s))
 
 let witness_value (#a:Type0) (b:ibuffer a)
   :HST.ST unit (requires (fun h0        -> True))
                (ensures  (fun h0 _ h1 -> h0 == h1 /\ b `value_is` (Ghost.hide (as_seq h1 b))))
   = let h = HST.get () in
     let s = Ghost.hide (as_seq h b) in
-    witness_p b (seq_eq s)
+    witness_p b (cpred s)
 
-let recall_value (#a:Type0) (b:ibuffer a) (s:Ghost.erased (Seq.seq a))
+let recall_value (#a:Type0) (b:ibuffer a) (s:eseq a)
   :HST.ST unit (requires (fun h0        -> (recallable b \/ live h0 b) /\ b `value_is` s))
                (ensures  (fun h0 _ h1 -> h0 == h1 /\ live h1 b /\ as_seq h1 b == Ghost.reveal s))
-  = recall_p b (seq_eq s)
+  = recall_p b (cpred s)
 
 (*
  * Immutable buffers are distinct from (trivial) buffers
